lean_backend/FastProofTheoryLogic.lean
@@ -1,0 +1,16 @@
+import FastProofTheory.ProofSystems.Rules
+import FastProofTheory.ProofSystems.Substructural
+import FastProofTheory.ProofSystems.IntuitionisticNaturalDeductionNJ
+import FastProofTheory.ProofSystems.ClassicalNaturalDeductionNK
+import FastProofTheory.ProofSystems.IntuitionisticSequentCalculusLJ
+import FastProofTheory.ProofSystems.ClassicalSequentCalculusLK
+import FastProofTheory.ProofSystems.Linear
+import FastProofTheory.ProofSystems.LinearSequentUrzyczyn
+import FastProofTheory.ProofSystems.IntuitionisticSequentCalculusLJMeta
+import FastProofTheory.Linear.Profile
+import FastProofTheory.Logic.IPC.Language
+import FastProofTheory.Logic.IPC.PropositionalND
+import FastProofTheory.Logic.IPC.FirstOrderND
+import FastProofTheory.Logic.IPC.Kripke
+import FastProofTheory.Logic.IPC.Heyting
+import FastProofTheory.Logic.IPC.Soundness
