lean_backend/Main.lean
@@ -1,4 +1,4 @@
-import FastProofTheory
+import FastProofTheoryBackend
 
 def main : IO Unit :=
   IO.println "fast-proof-theory"
